proof/schnorr_protocol/W64_SchnorrProtocol.ec
@@ -1,9 +1,12 @@
 require import AllCore.
 from Jasmin require import JModel.
 require import Array32 Array64 Array128.
-require export W64_SchnorrProver W64_SchnorrVerifier.
 
-type sbits.
+
+require import W64_SchnorrExtract.
+
+module JProver = M(Syscall).
+module JVerifier = M(Syscall).
 
 module type ZKProverJ = {
   proc response (witness0:W64.t Array32.t, secret_power:W64.t Array32.t,
@@ -48,6 +51,10 @@ module SoundnessJ(P:ZKMaliciousProverJ, V:ZKVerifierJ) = {
     return (v <> W64.zero);
   }
 }.
+
+
+
+type sbits.                     (* rewinding parameter type *)
 
 
 module type ZKRewindableMaliciousProverJ = {
