src/README.md
@@ -1,0 +1,1 @@
+stay tuned, so far try `make run`
